bn/BN_spec.v
@@ -1,0 +1,541 @@
+Require Import floyd.proofauto.
+Require Import Coqlib.
+Require Import Integers.
+Require Import List. Import ListNotations.
+Local Open Scope logic.
+
+Require Import sha.pure_lemmas.
+Require Import sha.common_lemmas.
+
+Require Import bn.minibn.
+Require Import BN_repr.
+
+(******************* From verif_queue etc ************************)
+
+Definition mallocN_spec :=
+ DECLARE _mallocN
+  WITH n: int
+  PRE [ 1%positive OF tint]
+     PROP (4 <= Int.signed n) 
+     LOCAL (temp 1%positive (Vint n))
+     SEP ()
+  POST [ tptr tvoid ] `(memory_block Tsh n) retval.
+
+(***********************From spec_sha**************************)
+(*
+Definition memcpy_spec :=
+  DECLARE _memcpy
+   WITH sh : share*share, p: val, q: val, n: Z, contents: list int 
+   PRE [ 1%positive OF tptr tvoid, 2%positive OF tptr tvoid, 3%positive OF tuint ]
+       PROP (writable_share (snd sh); 0 <= n <= Int.max_unsigned)
+       LOCAL (temp 1%positive p; temp 2%positive q; temp 3%positive (Vint (Int.repr n)))
+       SEP (`(data_at (fst sh) (tarray tuchar n) (map Vint contents) q);
+              `(memory_block (snd sh) (Int.repr n) p))
+    POST [ tptr tvoid ]
+         local (`(eq p) retval) &&
+       (`(data_at (fst sh) (tarray tuchar n) (map Vint contents) q) *
+        `(data_at (snd sh) (tarray tuchar n) (map Vint contents) p)).
+*)
+(***********************From spec_hmac*************************)
+
+Record TREP := mkTrep { t: type; v: reptype t}.
+Definition tp_of (T:TREP) : type.
+  destruct T. apply t0. 
+Defined.
+Definition v_of (T:TREP) : reptype (tp_of T).
+  destruct T. apply v0. 
+Defined.
+
+Definition memcpy_spec_data_at :=
+  DECLARE _memcpy
+   WITH sh : share*share, p: val, q: val, T:TREP
+   PRE [ 1%positive OF tptr tvoid, 2%positive OF tptr tvoid, 3%positive OF tuint ]
+       PROP (writable_share (snd sh); 0 <= sizeof  (tp_of T) <= Int.max_unsigned)
+       LOCAL (`(eq p) (eval_id 1%positive); `(eq q) (eval_id 2%positive);
+                    `(eq (Vint (Int.repr (sizeof (tp_of T))))) (eval_id 3%positive))
+       SEP (`(data_at (fst sh)  (tp_of T) (v_of T) q);
+              `(memory_block (snd sh) (Int.repr (sizeof  (tp_of T))) p))
+    POST [ tptr tvoid ]
+         local (`(eq p) retval) &&
+       (`(data_at (snd sh) (tp_of T) (v_of T) p) *`(data_at (fst sh) (tp_of T) (v_of T) q)).
+
+(******************************************************************)
+
+Definition bn_new: bnabs:= BNabs nil 0 0 false Int.zero.
+
+Definition bn_wexpand (A:bnabs) (w:int) : bnabs :=
+  match A with BNabs chun t dm ng fl =>
+    match nat_compare (Z.to_nat (Int.unsigned w)) dm with
+      Gt => BNabs chun t (Z.to_nat (Int.unsigned w)) ng fl
+    | _ => A
+  end
+  end.
+
+Definition bn_wexpand_spec :=
+  DECLARE _bn_wexpand
+   WITH b:val, B:bnabs, w:int
+   PRE [_bn OF tptr t_struct_bignum_st, _words OF tuint]
+       PROP ( Int.unsigned w < 16777215 )
+       LOCAL (temp _bn b; temp _words (Vint w))
+       SEP (`(bnstate_ B b))
+    POST [ tptr t_struct_bignum_st ] `(bnstate_ (bn_wexpand B w)) retval.
+Parameter myZ1:Z.
+
+Lemma body_bn_wexpand: semax_body nil (mallocN_spec ::memcpy_spec_data_at::nil)
+      f_bn_wexpand bn_wexpand_spec.
+Proof.
+start_function.
+name a _a.
+name a' _a'.
+unfold bnstate_; normalize. intros [d [top [dsize [neg flags]]]].
+destruct B as [DATA TOP DSIZE NEG FLAGS].
+unfold bn_relate; simpl. normalize.
+intros topN; normalize. intros dsizeN; normalize. intros dsN; normalize.
+(*unfold chunks_relate. normalize. intros TL. normalize.*)
+remember
+  (PROP  (Z.of_nat dsizeN < Int.unsigned w)
+   LOCAL  (temp _bn b; temp _words (Vint w))
+   SEP  (`(chunks_relate dsizeN DATA d);
+   `(data_at Tsh t_struct_bignum_st (d, (top, (dsize, (neg, flags)))) b))) as PST.
+
+forward_if PST.
+ subst. simpl. intros rho. entailer. simpl.  admit.
+
+forward. forward. entailer. (*solves the goal but why?*)
+  (* unfold POSTCONDITION, abbreviate. subst; simpl. intros rho. entailer.*)
+
+subst PST; normalize.
+remember
+  (PROP  ()
+   LOCAL  (temp _bn b; temp _words (Vint w))
+   SEP  (`(chunks_relate dsizeN DATA d);
+   `(data_at Tsh t_struct_bignum_st (d, (top, (dsize, (neg, flags)))) b))) as PST.
+rewrite HeqPST.
+forward_if PST.
+  forward. rewrite mul_repr in H7. simpl in H7.
+   rewrite Int.divs_pow2 with (logn:=Int.repr 7) in H7; try reflexivity.
+   unfold Int.ltu in H7.
+   destruct (zlt (Int.unsigned (Int.shrx (Int.repr 2147483647) (Int.repr 7)))
+           (Int.unsigned _id)). 2: discriminate.
+    unfold Int.shrx, Int.shl, Int.divs, Z.quot in l. simpl in l.
+    rewrite Int.unsigned_repr in l. omega.
+    rewrite int_max_unsigned_eq. omega.
+
+  forward. subst PST; simpl. intros rho. entailer.
+    
+subst PST; simpl.
+
+remember
+  (PROP  ()
+   LOCAL  (temp _bn b; temp _words (Vint w))
+   SEP  (`(chunks_relate dsizeN DATA d);
+   `(data_at Tsh t_struct_bignum_st (d, (top, (dsize, (neg, flags)))) b))) as PST.
+
+forward_if PST.
+ subst. simpl. intros rho.  entailer. simpl.  admit.
+
+forward. forward. entailer. 
+
+subst PST; normalize.
+assert (U: exists u, Int.mul (Int.repr 4) w = Int.repr u /\ 0 <= u <= Int.max_unsigned). admit. (*later*)
+destruct U as [u [U UBND]].
+forward_call (Int.repr u).
+  entailer!.
+  rewrite <- U; clear U. admit. (*later: exploit that 1<=w holds by H6*)
+after_call. clear a'0.
+forward.
+remember
+  (EX aval:val,
+   PROP  ()
+   LOCAL 
+   (temp _a aval;
+   temp _bn b; temp _words (Vint w))
+   SEP  (`(memory_block Tsh (Int.repr u)) (eval_id _a);
+   `(chunks_relate dsizeN DATA d);
+   `(data_at Tsh t_struct_bignum_st (d, (top, (dsize, (neg, flags)))) b))) as PST.
+forward_if PST.
+  forward. rename _id0 into i. unfold isptr in Pa'. 
+    destruct a'; simpl in *; try contradiction. inv H7.
+  forward. subst PST; simpl. intros rho; entailer.
+    remember (eval_id _a' rho) as aval.
+    unfold isptr in H9. destruct aval; simpl in *; try contradiction.
+    rewrite H2 in *. simpl in H1. 
+    apply (exp_right (Vptr b0 i)). unfold temp. entailer. rewrite H2. cancel.
+subst PST; normalize. apply extract_exists_pre. intros av.
+unfold chunks_relate. normalize. intros TL. normalize.
+rewrite <- H7 in *; clear H7.
+
+(*replace (eval_id _a) with av, so that we can use memory_block_split;
+  this was a bit more elegant before temp was introduced*)
+apply semax_pre with (P':=
+  (PROP  ()
+   LOCAL  (temp _a av; temp _bn b; temp _words (Vint w))
+   SEP 
+   (`(data_at Tsh (tarray tuint (Z.of_nat (length (DATA ++ TL))))
+        (map Vint (DATA ++ TL)) d);
+   `(memory_block Tsh (Int.repr u) av);
+   `(data_at Tsh t_struct_bignum_st (d, (top, (dsize, (neg, flags)))) b)))).
+  entailer.
+
+rewrite memory_block_isptr. normalize.
+destruct av; simpl in *; try contradiction. clear H7. rename b0 into av.
+assert (exists zz, u = (Z.of_nat (mult topN 4%nat)) + zz /\ 0 <= zz).
+  assert (Int.unsigned (Int.mul (Int.repr 4) w) = Int.unsigned (Int.repr u)).
+    rewrite U; trivial.
+  rewrite Int.unsigned_repr in H7; trivial.
+  subst u. exists (Zmult (Int.unsigned w - Z.of_nat topN) 4).
+  rewrite Nat2Z.inj_mul. simpl.
+  rewrite Z.mul_sub_distr_r, Zplus_minus.
+  simpl. 
+  specialize (mul_repr 4 (Int.unsigned w)).
+  rewrite Int.repr_unsigned. intros IM; rewrite IM; clear IM.
+   rewrite Z.mul_comm.
+   rewrite Int.unsigned_repr. split; trivial. omega. 
+   rewrite int_max_unsigned_eq. omega.
+destruct H7 as [zz [ZZ ZZpos]]. subst u.
+specialize (memory_block_split Tsh av (Int.unsigned i) (Z.of_nat (mult topN 4%nat)) zz).
+rewrite Int.repr_unsigned. intros MBS.
+rewrite MBS; trivial; clear MBS.
+Focus 2. omega.
+Focus 2. rewrite <-initialize.max_unsigned_modulus. omega.
+normalize. unfold tarray. rewrite H2.
+unfold_data_at 1%nat.
+unfold field_at. simpl. normalize. SearchAbout array_at'. simpl. specify memcpy now on array_at'??
+erewrite field_at_Tarray. 2: reflexivity. 2: apply JMeq.JMeq_refl.
+SearchAbout array_at. unfold Tarray.
+specialize split2_array_at0 TSh .
+specialize (data_at_Tarray_split3 Tsh tuint). 
+(Z.of_nat (dsN * 4)) noattr (Z.of_nat (topN * 4))).
+ (*(Z.of_nat (topN * 4))*)
+remember (mkTrep (tarray tuint myZ1) (map Vint (DATA ++ TL))) as W.
+
+remember ((Tsh, Tsh), Vptr av i, d, W) as WIT.
+(*remember ((Tsh, Tsh), Vptr av i, d, Z.of_nat mx, ch ++ TL) as WIT.*)
+forward_call WIT.
+ { assert (FR: Frame = [`(data_at Tsh t_struct_bignum_st (d, (top, (dsize, (neg, flags)))) b);
+                        `(memory_block Tsh (Int.repr zz)
+    (Vptr av (Int.repr (Int.unsigned i + Z.of_nat (mult topN 4%nat)))))]).
+     subst Frame. reflexivity. 
+   rewrite FR. clear FR Frame. 
+   subst WIT. simpl. intros rho. entailer. simpl.
+   destruct d; simpl in *; try contradiction.
+   rewrite Z.max_comm. (* initialize.Zmax_Z_of_nat.*)
+   apply andp_right.
+   apply prop_right. admit. (*later*)
+   cancel.  rewrite Z.max_comm, initialize.Zmax_Z_of_nat.
+   erewrite (data_at_type_changable _ _ (tarray tuchar (Z.of_nat (length (ch ++ TL))))).
+    apply derives_refl.
+
+
+admit.
+
+omega.
+assert (exists zz, w4 = (Z.of_nat mx) + zz). admit.
+destruct H6 as [zz ZZ]. subst w4.
+specialize (memory_block_split Tsh av (Int.unsigned i) (Z.of_nat mx) zz).
+rewrite Int.repr_unsigned; intros.
+rewrite H6; clear H6.
+normalize.
+remember (mkTrep (tarray tuint (Z.of_nat mx)) (map Vint (ch ++ TL))) as W.
+
+remember ((Tsh, Tsh), Vptr av i, d, W) as WIT.
+(*remember ((Tsh, Tsh), Vptr av i, d, Z.of_nat mx, ch ++ TL) as WIT.*)
+forward_call WIT.
+ { assert (FR: Frame = [`(data_at Tsh t_struct_bignum_st (d, (t, (m, (n, f)))) b);
+                        `(memory_block Tsh (Int.repr zz)
+                          (Vptr av (Int.repr (Int.unsigned i + Z.of_nat mx))))]).
+     subst Frame. reflexivity. 
+   rewrite FR. clear FR Frame. 
+   subst WIT. simpl. intros rho. entailer. simpl.
+   destruct d; simpl in *; try contradiction.
+   apply andp_right.
+   apply prop_right. admit. (*later*)
+   cancel.  rewrite Z.max_comm, initialize.Zmax_Z_of_nat.
+   erewrite (data_at_type_changable _ _ (tarray tuchar (Z.of_nat (length (ch ++ TL))))).
+    apply derives_refl.
+   simpl. unfold tarray. simpl. unfold tuchar, tuint.
+      rewrite Z.max_comm, initialize.Zmax_Z_of_nat.
+      remember (Z.of_nat (length (ch ++ TL))) as l. SearchAbout Z.max 0.  ext. cancel. 
+   instantiate (1:=nil). subst WIT; simpl.
+remember ((Tsh,Tsh), 
+frame_SEP 2.
+remember (mkTrep (tarray tuint (4 * Z.of_nat mx)) (map Vint (ch ++ TL))) as W.
+remember ((Tsh, Tsh), av, d, W) as WIT.
+eapply semax_seq'.
+forward_call WIT.
+ { assert (FR: Frame = nil).  subst Frame. reflexivity. 
+   rewrite FR. clear FR Frame. 
+   subst WIT W. simpl. ; intros. entailer. simpl.
+   destruct av; simpl in *; try contradiction.
+   destruct d; simpl in *; try contradiction.
+   apply andp_right.
+   apply prop_right. split. admit. (*later*)
+      rewrite Z.max_comm, initialize.Zmax_Z_of_nat.
+      remember (Z.of_nat (length (ch ++ TL))) as l. SearchAbout Z.max 0.  ext. cancel. 
+   instantiate (1:=nil). subst WIT; simpl.
+remember ((Tsh,Tsh), 
+frame_SEP 2.
+
+ isubst PST; simpl. intros rho; entailer!.  normalize. simpl in H6. unfold is_pointer_or_null in TC1. 
+    remember (force_val (sem_cast_neutral a')) as q.
+    destruct q; try contradiction. subst; simpl in *.
+unfold isptr in Pa'. destruct a'; simpl in *. inv Heqq.
+      unfold typed_true in H6. simpl in H6.
+       destruct TC1. unfold sem_cmp_pp in H6. SearchAbout typed_true tint sem_cmp_pp. 
+
+   rewrite Int.mul_signed.
+   assert (1 <= Int.unsigned w). omega.
+   rewrite Int.mul_signed.
+rewrite Int.signed_repr.
+rewrite Int.signed_repr.
+rewrite Int.signed_eq_unsigned. omega. unfold Int.max_signed. simpl. omega.
+unfold Int.max_signed, Int.min_signed. simpl. omega.
+unfold Int.max_signed, Int.min_signed. simpl. omega.
+forward_seq.
+forward_seq.
+forward_call WIT.
+  entailer!.
+
+intros. simpl. intros rho. simpl.
+
+ SearchAbout Int.shl Int.one. Int.shl. simpl in l.  rewrite ltu_repr in H7. shrx. Focus 2. unfold Int.is_power2. reflexivity. simpl. simpl.  unfold Int.divs in H7. SearchAbout rewrite div_repr in H7. SearchAbout Int.mul. unfold Int.mul in H7. simpl.  unfold chunks_relate.  SearchAbout Int.ltu. unfold chunks_relate. SearchAbout Int.divs. Int.mul.
+
+SearchAbout temp.
+unfold temp in H6.
+unfold both_int in H4. unfold temp, liftx in *. simpl in *.
+unfold sem_cast_neutral in H4.
+SearchAbout typed_false.
+   simpl in H4.
+forward_seq.
+
+Definition bn_new: bnabs:= BNabs nil 0 0 false Int.zero.
+
+Definition bn_new_spec :=
+  DECLARE _BN_new
+   WITH u:unit
+   PRE []
+       PROP ()
+       LOCAL ()
+       SEP ()
+    POST [ tptr t_struct_bignum_st ] `(bnstate_ bn_new) retval.
+
+Lemma body_bn_new: semax_body nil (malloc_spec ::nil)
+      f_BN_new bn_new_spec.
+Proof.
+start_function.
+forward_seq.
+forward_seq.
+admit. (*forward_call (Int.repr 20).
+     assert (XX1: (var_types Delta) ! _malloc = None) 
+        by (reflexivity || fail 4 "The function-identifier " id " is not a global variable").
+    assert (match (glob_specs Delta) ! _malloc with
+               | Some (mk_funspec _ t _ _) => Some t
+               | _ => None
+               end = None);
+     simpl.*)
+forward_call (Int.repr 20).
+apply seq_assoc.
+apply seq_assoc. Check (Int.repr 20).
+remember (Int.repr 20) as WIT.
+forward_call WIT.
+forward_call (Int.repr 20).
+unfold bnstate_; normalize. intros av. normalize. intros bv. normalize.
+forward.
+  entailer. unfold bn_relate. destruct A as [d t dm n].
+   destruct av as [d' [t' [dm' [n' X]]]]. simpl. unfold tops_relate. normalize.
+forward.
+  entailer. unfold bn_relate. destruct B as [d t dm n].
+   destruct bv as [d' [t' [dm' [n' X]]]]. simpl. unfold tops_relate. normalize.
+forward.
+remember (PROP  ()
+   LOCAL  (temp _btop (fst (snd bv)); temp _atop (fst (snd av));
+   `(eq a) (eval_id _a); `(eq b) (eval_id _b))
+   SEP  (`(bn_relate A av); `(data_at Tsh t_struct_bignum_st av a);
+   `(bn_relate B bv); `(data_at Tsh t_struct_bignum_st bv b))) as PST.
+forward_if PST.
+  subst PST; normalize. 
+  forward. simpl in *.
+   apply andp_right.
+     unfold bn_ucmp. simpl. 
+     destruct A as [dA tA dmA nA]. destruct av as [dA' [tA' [dmA' [nA' XA]]]].
+     destruct B as [dB tB dmB nB]. destruct bv as [dB' [tB' [dmB' [nB' XB]]]].
+     simpl in *. unfold chunks_relate. normalize. admit.
+  unfold bnstate_. normalize. apply (exp_right bv). normalize.
+   apply (exp_right av). normalize.
+
+forward. subst PST. entailer.
+
+subst PST; normalize.
+forward. entailer. unfold bn_relate. destruct A as [d t dm n].
+   destruct av as [d' [t' [dm' [n' X]]]]. simpl. unfold chunks_relate. entailer.
+forward. entailer. unfold bn_relate. destruct B as [d t dm n].
+   destruct bv as [d' [t' [dm' [n' X]]]]. simpl. unfold chunks_relate. normalize.
+   destruct A as [dA tA dmA nA].
+   destruct av as [dA' [tA' [dmA' [nA' XA]]]]. simpl. unfold chunks_relate. entailer.
+continue here
+destruct A as [d t dm n].
+   destruct av as [d' [t' [dm' [n' X]]]]. simpl. unfold chunks_relate. entailer.
+
+ normalize.
+forward.
+  entailer. unfold bn_relate. destruct B as [d t dm n].
+   destruct bv as [d' [t' [dm' [n' X]]]]. simpl. unfold tops_relate. normalize.
+forward.
+ unfold bnstate_. entailer.  normalize. unfold POSTCONDITION, abbreviate. 
+  unfold bnstate_. entailer.
+  (dB',
+  (Vint (Int.repr (Z.of_nat (length dB))),
+  (Vint (Int.repr (Z.of_nat dmB)), (nB', XB))))). entailer. 
+  apply (exp_right  (dA',
+  (Vint (Int.repr (Z.of_nat (length dA))),
+  (Vint (Int.repr (Z.of_nat dmA)), (nA', XA))))). entailer.
+  unfold bn_relate. entailer. unfold tops_relate. entailer.
+destruct A as [dA tA dmA nA]. destruct av as [dA' [tA' [dmA' [nA' XA]]]].
+destruct B as [dB tB dmB nB]. destruct bv as [dB' [tB' [dmB' [nB' XB]]]].
+simpl. normalize. unfold tops_relate in *. subst tA' tB' dmA' dmB'.
+simpl.
+remember (Int.sub (Int.repr (Z.of_nat tA)) (Int.repr (Z.of_nat tB))) as i. 
+remember ((PROP  ( i <> Int.zero)
+   LOCAL  (temp _i (Vint i); temp _btop (Vint (Int.repr (Z.of_nat tB)));
+   temp _atop (Vint (Int.repr (Z.of_nat tA))); `(eq a) (eval_id _a);
+   `(eq b) (eval_id _b))
+   SEP  (`(chunks_relate dA dA');
+   `(data_at Tsh t_struct_bignum_st
+       (dA',
+       (Vint (Int.repr (Z.of_nat tA)),
+       (Vint (Int.repr (Z.of_nat dmA)), (nA', XA)))) a);
+   `(chunks_relate dB dB');
+   `(data_at Tsh t_struct_bignum_st
+       (dB',
+       (Vint (Int.repr (Z.of_nat tB)),
+       (Vint (Int.repr (Z.of_nat dmB)), (nB', XB)))) b)))) as PST.
+forward_if PST.
+  subst PST; normalize. 
+  forward. simpl in *.
+   apply andp_right.
+     unfold bn_ucmp. simpl. unfold chunks_relate. admit.
+  unfold bnstate_. normalize. apply (exp_right  (dB',
+  (Vint (Int.repr (Z.of_nat (length dB))),
+  (Vint (Int.repr (Z.of_nat dmB)), (nB', XB))))). entailer. 
+  apply (exp_right  (dA',
+  (Vint (Int.repr (Z.of_nat (length dA))),
+  (Vint (Int.repr (Z.of_nat dmA)), (nA', XA))))). entailer.
+  unfold bn_relate. entailer. unfold tops_relate. entailer.
+normalize.
+forward. entailer. rewrite H2, H3 in *. simpl in *. inv H1.
+  apply (exp_right (Int.sub _id1 _id0)). entailer.
+  destruct A as [dA tA dmA nA]. destruct av as [dA' [tA' [dmA' [nA' XA]]]].
+  destruct B as [dB tB dmB nB]. destruct bv as [dB' [tB' [dmB' [nB' XB]]]].
+  unfold bn_relate. entailer. simpl in *. subst. admit.
+
+   temp _btop (fst (snd bv)); temp _atop (fst (snd av));
+   `(eq a) (eval_id _a); `(eq (Vint i)) (eval_id _i); `(eq b) (eval_id _b))
+   SEP  (`(bn_relate A av); `(data_at Tsh t_struct_bignum_st av a);
+   `(bn_relate B bv); `(data_at Tsh t_struct_bignum_st bv b)))) as PST.
+forward_if PST.
+  subst; normalize. 
+  forward. simpl in *. rewrite H1, H2 in *. simpl in *. inv H0.
+   apply andp_right.
+     unfold bn_relate. destruct A as [dA tA dmA nA].
+     destruct av as [dA' [tA' [dmA' [nA' XA]]]]. destruct B as [dB tB dmB nB].
+     destruct bv as [dB' [tB' [dmB' [nB' XB]]]]. entailer. simpl in *. subst.
+     unfold bn_ucmp. simpl. unfold chunks_relate. admit.
+  unfold bnstate_. normalize. apply (exp_right bv). entailer.
+    apply (exp_right av). entailer.
+normalize.
+forward. entailer. rewrite H2, H3 in *. simpl in *. inv H1.
+  apply (exp_right (Int.sub _id1 _id0)). entailer.
+  destruct A as [dA tA dmA nA]. destruct av as [dA' [tA' [dmA' [nA' XA]]]].
+  destruct B as [dB tB dmB nB]. destruct bv as [dB' [tB' [dmB' [nB' XB]]]].
+  unfold bn_relate. entailer. simpl in *. subst. admit.
+
+subst.
+
+forward_seq.
+subst. forward. apply extract_exists. exp_left. forward.
+eapply semax_seq'.
+ensure_normal_ret_assert;
+ hoist_later_in_pre.
+Print t_struct_bignum_st.
+match goal with
+| SE := @abbreviate type_id_env.type_id_env _ 
+    |- semax ?Delta (|> (PROPx ?P (LOCALx ?Q (SEPx ?R)))) (Sset _ ?e) _ =>
+ (* Super canonical load *)
+    let e1 := fresh "e" in
+    let efs := fresh "efs" in
+    let tts := fresh "tts" in
+      construct_nested_efield e e1 efs tts;
+
+    let lr := fresh "lr" in
+      pose (compute_lr e1 efs) as lr;
+      vm_compute in lr;
+
+    let HLE := fresh "H" in
+    let p := fresh "p" in evar (p: val);
+      match goal with
+      | lr := LLLL |- _ => do_compute_lvalue Delta P Q R e1 p HLE
+      | lr := RRRR |- _ => do_compute_expr Delta P Q R e1 p HLE
+      end;
+
+    let H_Denote := fresh "H" in
+    let gfs := fresh "gfs" in
+      solve_efield_denote Delta P Q R efs gfs H_Denote
+end.
+;
+
+    let sh := fresh "sh" in evar (sh: share);
+    let t_root := fresh "t_root" in evar (t_root: type);
+    let gfs0 := fresh "gfs" in evar (gfs0: list gfield);
+    let v := fresh "v" in evar (v: reptype (nested_field_type2 t_root gfs0));
+    let n := fresh "n" in
+    let H := fresh "H" in
+    let H_LEGAL := fresh "H" in
+    sc_new_instantiate SE P Q R R Delta e1 gfs tts lr p sh t_root gfs0 v n (0%nat) H H_LEGAL
+end.
+;
+    
+    let gfs1 := fresh "gfs" in
+    let efs0 := fresh "efs" in
+    let efs1 := fresh "efs" in
+    let tts0 := fresh "tts" in
+    let tts1 := fresh "tts" in
+    let len := fresh "len" in
+    pose ((length gfs - length gfs0)%nat) as len;
+    simpl in len;
+    match goal with
+    | len := ?len' |- _ =>
+      pose (firstn len' gfs) as gfs1;
+      pose (skipn len' efs) as efs0;
+      pose (firstn len' efs) as efs1;
+      pose (skipn len' tts) as tts0;
+      pose (firstn len' tts) as tts1
+    end;
+    clear len;
+    unfold gfs, efs, tts in gfs0, gfs1, efs0, efs1, tts0, tts1;
+    simpl firstn in gfs1, efs1, tts1;
+    simpl skipn in gfs0, efs0, tts0;
+
+    change gfs with (gfs1 ++ gfs0) in *;
+    change efs with (efs1 ++ efs0) in *;
+    change tts with (tts1 ++ tts0) in *;
+    subst gfs efs tts p;
+
+    let Heq := fresh "H" in
+    match type of H with
+    | (PROPx _ (LOCALx _ (SEPx (?R0 :: nil))) 
+           |-- _) => assert (nth_error R n = Some R0) as Heq by reflexivity
+    end;
+    eapply (semax_SC_field_load Delta sh SE n) with (lr0 := lr) (t_root0 := t_root) (gfs2 := gfs0) (gfs3 := gfs1);
+    [reflexivity | reflexivity | reflexivity
+    | reflexivity | reflexivity | exact Heq | exact HLE | exact H_Denote 
+    | exact H | reflexivity
+    | try solve [entailer!]; try (clear Heq HLE H_Denote H H_LEGAL;
+      subst e1 gfs0 gfs1 efs1 efs0 tts1 tts0 t_root v sh lr n; simpl app; simpl typeof)
+    | solve_legal_nested_field_in_entailment; try clear Heq HLE H_Denote H H_LEGAL;
+      subst e1 gfs0 gfs1 efs1 efs0 tts1 tts0 t_root v sh lr n]
+end.
+
+
+forward.
+  entailer.
+
